Further developments for ZXbiperm

src/Relations/ZXbiperm.v
@@ -5,6 +5,7 @@ Import CastRules.
 From QuantumLib Require Import Bits.
 Require Export QuantumLib.Permutations.
 Import QuantumLib.VectorStates Modulus Kronecker.
+Require Import ZXpermAutomation ZXpermFacts.
 Require Import NFBiperm.
 
 
@@ -200,6 +201,591 @@ Proof.
     now apply kron_mat_prop_proper.
 Qed.
 
+Notation biperm_of_zx zx := (realize_NF_biperm (NF_of_zx zx)).
+
+Lemma ZXbiperm_prop_by_biperm_eq {n m} (zx0 zx1 : ZX n m) 
+  (Hzx0 : ZXbiperm zx0) (Hzx1 : ZXbiperm zx1) : 
+  perm_eq (m + n) (biperm_of_zx zx0) (biperm_of_zx zx1) ->
+  zx0 ∝ zx1.
+Proof.
+  intros Heq.
+  change (⟦zx0⟧ [∝] ⟦zx1⟧).
+  rewrite 2!NF_of_zx_correct by easy.
+  unfold matrix_of_NF_biperm.
+  rewrite !NF_insize_NF_of_zx, !NF_outsize_NF_of_zx by assumption.
+  erewrite matrix_of_biperm_eq_of_perm_eq;
+  [|rewrite Nat.add_comm; apply Heq].
+  easy.
+Qed.
+
+(* Automation and specific instances *)
+
+Lemma zxbiperm_cast {n m n' m'} (zx : ZX n m) prfn prfm : 
+  ZXbiperm zx -> ZXbiperm (cast n' m' prfn prfm zx).
+Proof.
+  now subst.
+Qed.
+
+Create HintDb zxbiperm_db discriminated.
+
+#[export] Hint Constructors ZXbiperm : zxbiperm_db.
+#[export] Hint Resolve zxbiperm_cast : zxbiperm_db.
+(* Makes it handle dimensions better, particularly 
+  for small, concrete examples: *)
+#[export] Hint Extern 0 (ZXbiperm (_ ⟷ _)) =>
+  apply BipermCompose : zxbiperm_db.
+#[export] Hint Extern 0 (ZXbiperm (?zx0 ↕ ?zx1)) =>
+  match type of zx0 with
+  | ZX ?n0 ?m0 =>
+  match type of zx1 with
+  | ZX ?n1 ?m1 =>
+  apply (@BipermStack _ _ _ _ zx0 zx1)
+  end end : zxbiperm_db.
+
+Lemma zxperm_zxbiperm {n} (zx : ZX n n) : ZXperm n zx -> ZXbiperm zx.
+Proof.
+  intros H.
+  induction H; auto with zxbiperm_db.
+Qed.
+
+(* NB for this to do anything, zxperm_db will have to be used
+   as well, e.g. auto with zxbiperm_db zxperm_db *)
+#[export] Hint Resolve zxperm_zxbiperm : zxbiperm_db.
+
+Lemma transpose_zxbiperm {n m} (zx : ZX n m) (H : ZXbiperm zx) :
+  ZXbiperm (ZXCore.transpose zx).
+Proof.
+  induction H; cbn; auto with zxbiperm_db.
+Qed.
+
+Lemma colorswap_zxbiperm {n m} (zx : ZX n m) (H : ZXbiperm zx) :
+  ZXbiperm (⊙ zx).
+Proof.
+  induction H; cbn; auto with zxbiperm_db.
+Qed.
+
+Lemma adjoint_zxbiperm {n m} (zx : ZX n m) (H : ZXbiperm zx) :
+  ZXbiperm (ZXCore.adjoint zx).
+Proof.
+  induction H; cbn; auto with zxbiperm_db.
+Qed.
+
+#[export] Hint Resolve transpose_zxbiperm 
+  colorswap_zxbiperm adjoint_zxbiperm : zxbiperm_db.
+
+Lemma n_stack_zxbiperm {m o} (zx : ZX m o) n (H : ZXbiperm zx) : 
+  ZXbiperm (n ⇑ zx).
+Proof.
+  induction n; cbn; auto with zxbiperm_db.
+Qed.
+
+#[export] Hint Resolve n_stack_zxbiperm : zxbiperm_db.
+
+
+Lemma n_stacked_pf_1 {n} : n + n = n * 2. Proof. lia. Qed.
+Lemma n_stacked_pf_2 {n} : 0 = n * 0. Proof. lia. Qed.
+Definition n_stacked_caps n : ZX (n + n) 0 :=
+  cast _ _ n_stacked_pf_1 n_stacked_pf_2 (n ⇑ ⊃).
+
+Definition n_stacked_cups n : ZX 0 (n + n) :=
+  cast _ _ n_stacked_pf_2 n_stacked_pf_1 (n ⇑ ⊂).
+
+Lemma n_stacked_caps_zxbiperm n : 
+  ZXbiperm (n_stacked_caps n).
+Proof. 
+  unfold n_stacked_caps. 
+  auto with zxbiperm_db.
+Qed.
+
+Lemma n_stacked_cups_zxbiperm n : 
+  ZXbiperm (n_stacked_cups n).
+Proof. 
+  unfold n_stacked_cups. 
+  auto with zxbiperm_db.
+Qed.
+
+#[export] Hint Resolve n_stacked_caps_zxbiperm 
+  n_stacked_cups_zxbiperm : zxbiperm_db.
+
+Lemma n_stack_semantics {n m} (zx : ZX n m) k : 
+  ⟦ k ⇑ zx ⟧ = kron_n k (⟦ zx ⟧).
+Proof.
+  induction k; [easy|].
+  rewrite kron_n_assoc by auto_wf.
+  cbn.
+  f_equal;
+  [rewrite Nat.mul_comm; apply Nat.pow_mul_r..|].
+  easy.
+Qed.
+
+Lemma n_stacked_caps_semantics n : 
+  ⟦ n_stacked_caps n ⟧ = kron_n n (⟦ ⊃ ⟧).
+Proof.
+  unfold n_stacked_caps.
+  rewrite cast_semantics_dim.
+  unfold cast_semantics_dim_eqn.
+  apply n_stack_semantics.
+Qed.
+
+Lemma n_stacked_cups_semantics n : 
+  ⟦ n_stacked_cups n ⟧ = kron_n n (⟦ ⊂ ⟧).
+Proof.
+  unfold n_stacked_cups.
+  rewrite cast_semantics_dim.
+  unfold cast_semantics_dim_eqn.
+  apply n_stack_semantics.
+Qed.
+
+Definition zx_of_NF_uncasted (b : NF_biperm) : 
+  ZX (NF_insize b) (NF_outsize b) :=
+  zx_of_perm (NF_insize b) (lperm' b) ⟷
+    ((n_stacked_caps (ncup' b) ⟷ n_stacked_cups (ncap' b)) 
+    ↕ n_wire (nid' b)) ⟷
+  zx_of_perm (NF_outsize b) (rperm' b).
+
+Lemma zx_of_NF_uncasted_semantics b (Hb : WF_NF_biperm b) : 
+  ⟦ zx_of_perm (NF_insize b) (lperm' b) ⟷
+      ((n_stacked_caps (ncup' b) ⟷ n_stacked_cups (ncap' b)) 
+      ↕ n_wire (nid' b)) ⟷
+    zx_of_perm (NF_outsize b) (rperm' b) ⟧ = 
+  matrix_of_NF_biperm b.
+Proof.
+  cbn [ZX_semantics].
+  rewrite 2!zx_of_perm_semantics by apply Hb.
+  rewrite n_stacked_cups_semantics, n_stacked_caps_semantics.
+  rewrite matrix_of_WF_NF_biperm by easy.
+  rewrite matrix_of_biperm_n_m_cup_cap, n_wire_semantics.
+  rewrite Mmult_assoc.
+  easy.
+Qed.
+
+Lemma zx_of_NF_uncasted_zxbiperm b : 
+  ZXbiperm (zx_of_NF_uncasted b).
+Proof.
+  unfold zx_of_NF_uncasted.
+  auto with zxbiperm_db zxperm_db.
+Qed.
+
+#[export] Hint Resolve zx_of_NF_uncasted_zxbiperm : zxbiperm_db.
+
+Definition zx_of_bipermutation n m f 
+  (Hf : bipermutation (m + n) f) : ZX n m :=
+  cast _ _ 
+    (eq_sym (NF_insize_NF_of_biperm n m f Hf))
+    (eq_sym (NF_outsize_NF_of_biperm n m f Hf))
+    (zx_of_NF_uncasted (NF_of_biperm n m f)).
+
+(* FIXME: Move *)
+Definition true_rel {A} : relation A :=
+  fun _ _ => True.
+
+Instance true_rel_superrel {A} (R : relation A) : 
+  subrelation R true_rel.
+Proof.
+  intros x y H.
+  constructor.
+Qed.
+
+Add Parametric Morphism n m f : (zx_of_bipermutation n m f) 
+  with signature
+  true_rel ==> eq as 
+  zx_of_bipermutation_proper.
+Proof.
+  intros H H' _.
+  unfold zx_of_bipermutation.
+  f_equal; 
+  apply Peano_dec.UIP_nat.
+Qed.
+
+Definition bipermutation_dec n f : 
+  {bipermutation n f} + {~ bipermutation n f}.
+Proof.
+  destruct (permutation_dec f n);
+  [|right; rewrite bipermutation_defn_alt; tauto].
+  destruct (perm_eq_dec n (perm_inv n f) f);
+  [|right; rewrite bipermutation_defn_alt; tauto].
+  destruct (bool_dec (forallb (fun k => negb (f k =? k)) 
+    (seq 0 n)) true) as [e | e];
+  rewrite forallb_seq0 in e;
+  setoid_rewrite negb_true_iff in e;
+  setoid_rewrite Nat.eqb_neq in e;
+  [left | right];
+  rewrite bipermutation_defn_alt;
+  tauto.
+Qed.
+
+Definition zx_dummy n m : ZX n m :=
+  Z n m 0.
+
+Global Opaque zx_dummy.
+
+Definition zx_of_biperm n m f :=
+  match bipermutation_dec (m + n) f with 
+  | left Hf => zx_of_bipermutation n m f Hf
+  | right _ => zx_dummy n m
+  end.
+
+Lemma n_cup_unswapped_zxbiperm n : ZXbiperm (n_cup_unswapped n).
+Proof.
+  induction n; cbn -[Nat.add]; auto with zxbiperm_db.
+Qed.
+
+#[export] Hint Resolve n_cup_unswapped_zxbiperm : zxbiperm_db.
+
+Lemma n_cup_zxbiperm n : ZXbiperm (n_cup n).
+Proof.
+  unfold n_cup.
+  auto with zxbiperm_db zxperm_db.
+Qed.
+
+#[export] Hint Resolve n_cup_zxbiperm : zxbiperm_db.
+
+Lemma n_cap_zxbiperm n : ZXbiperm (n_cap n).
+Proof.
+  unfold n_cap; auto with zxbiperm_db.
+Qed.
+
+#[export] Hint Resolve n_cap_zxbiperm : zxbiperm_db.
+
+
+
+Lemma kron_f_to_vec_eq {n m p q : nat} (A : Matrix (2^n) (2^m))
+  (B : Matrix (2^p) (2^q)) (f : nat -> bool) : WF_Matrix A -> WF_Matrix B -> 
+  A ⊗ B × f_to_vec (m + q) f
+  = A × f_to_vec m f ⊗ (B × f_to_vec q (fun k : nat => f (m + k))).
+Proof.
+  intros.
+  prep_matrix_equivalence.
+  apply kron_f_to_vec.
+Qed.
+
+Lemma realize_NF_biperm_spec b (Hb : WF_NF_biperm b) :
+  perm_eq (NF_outsize b + NF_insize b) 
+    (realize_NF_biperm b) 
+    (stack_perms (NF_outsize b) (NF_insize b) 
+      (reflect_perm (NF_outsize b) ∘ perm_inv (NF_outsize b) (rperm' b) 
+        ∘ reflect_perm (NF_outsize b))
+      (reflect_perm (NF_insize b) ∘ lperm' b
+        ∘ reflect_perm (NF_insize b)) ∘
+      stack_biperms (nid' b) (nid' b) (ncap' b + ncap' b) (ncup' b + ncup' b)
+      (idn_biperm (nid' b)) (n_m_cup_cap (ncup' b) (ncap' b)) ∘
+    stack_perms (NF_outsize b) (NF_insize b) 
+      (reflect_perm (NF_outsize b) ∘ rperm' b
+        ∘ reflect_perm (NF_outsize b))
+      (reflect_perm (NF_insize b) ∘ perm_inv (NF_insize b) (lperm' b)
+        ∘ reflect_perm (NF_insize b))).
+Proof.
+  unfold realize_NF_biperm, uncurry_NF_biperm.
+  unfold realize_biperm_data.
+  rewrite biperm_compose_perm_l_spec.
+  destruct Hb.
+  rewrite biperm_compose_perm_r_spec by auto with biperm_db.
+  rewrite !compose_assoc, stack_perms_compose, 
+    <- ! compose_assoc, stack_perms_compose by auto with perm_bounded_db.
+  rewrite 2!compose_idn_l, 2!compose_idn_r.
+  rewrite !perm_inv_compose by auto with perm_db.
+  repeat rewrite reflect_perm_inv at 1.
+  rewrite perm_inv_perm_inv by auto with perm_db.
+  easy.
+Qed.
+
+Lemma div_eq a b : a / b = (a - a mod b) / b.
+Proof.
+  rewrite (Nat.div_mod_eq a b) at 2.
+  rewrite Nat.add_sub.
+  bdestruct (b =? 0).
+  - now subst.
+  - now rewrite Nat.mul_comm, Nat.div_mul by easy.
+Qed.
+
+(* Search Nat.modulo Nat.sub. *)
+Lemma div_sub a b c : c <> 0 -> 
+  (b * c - a) / c = b - a / c - Nat.b2n (¬ a mod c =? 0).
+Proof.
+  intros Hc.
+  bdestruct (a <? b * c); cycle 1.
+  - replace (b * c - a) with 0 by lia.
+    rewrite Nat.Div0.div_0_l.
+    pose proof (Nat.div_le_lower_bound a c b); lia.
+  - assert (a / c < b) by show_moddy_lt.
+    apply (Nat.mul_cancel_r _ _ c Hc).
+    rewrite div_mul_not_exact by easy.
+    rewrite 2!Nat.mul_sub_distr_r.
+    rewrite div_mul_not_exact by easy.
+    pose proof (Nat.mod_le (b * c - a) c Hc).
+    pose proof (Nat.mod_le a c Hc).
+    enough (a + (b * c - a) mod c = 
+      (a + c * Nat.b2n (¬ a mod c =? 0) - a mod c))
+      by lia.
+    rewrite <- Nat.add_sub_assoc by 
+      (pose proof (Nat.mod_upper_bound a c Hc);
+      bdestructΩ'; cbn; lia).
+    f_equal.
+    Abort.
+
+
+
+Lemma kron_comm_perm_2_n_conj_reflect_perm_eq n : 
+  reflect_perm (n + n) ∘ kron_comm_perm 2 n ∘ reflect_perm (n + n) = 
+  kron_comm_perm 2 n.
+Proof.
+  replace (n + n) with (2 * n) by lia.
+  eq_by_WF_perm_eq (2 * n).
+  do 2 rewrite reflect_perm_defn at 1.
+  rewrite kron_comm_perm_defn.
+  unfold compose.
+  intros k Hk.
+  Abort.
+
+
+Lemma reflect_perm_NF_rep n : 
+  is_NF_representative (n + n) (n + n) 
+    {| lperm' := idn; rperm' := kron_comm_perm 2 n;
+      ncup' := 0; ncap' := n; nid' := 0|} (reflect_perm (n + n)).
+Proof.
+  split.
+  split; cbn; auto with perm_db; 
+  eapply permutation_change_dims; [| auto with perm_db]; lia.
+  split; split; [cbn; lia..|].
+  rewrite realize_NF_biperm_constructor.
+  unfold realize_biperm_data.
+  eapply perm_eq_dim_change_if_nonzero;
+  [rewrite biperm_compose_perm_l_spec|lia].
+  rewrite biperm_compose_perm_r_spec by auto with biperm_db.
+  rewrite compose_assoc.
+  cleanup_perm.
+  zarith.
+  eapply permutation_change_dims; [|auto with perm_db];
+   solve [eauto with perm_db zarith].
+  Abort.
+
+Lemma n_cup_unswapped_semantics n : 
+  ⟦ n_cup_unswapped n ⟧ = 
+  matrix_of_biperm 0 (n + n) 
+    (reflect_perm (n + n)).
+Proof.
+  induction n.
+  - cbn.
+    now rewrite matrix_of_biperm_0_0.
+  - cbn.
+    simpl_rewrite' matrix_of_cap_NF_biperm.
+Abort.
+
+
+
+(* FIXME: These lemmas go in BipermutationMatrices.v *)
+
+Lemma number_preserved_0 f n : 
+  number_preserved 0 f n = true.
+Proof.
+  rewrite number_preserved_iff_all_lt_eq.
+  intros; now rewrite 2!Nat.bits_0.
+Qed.
+
+Lemma matrix_of_biperm_entry_0_0 n m f : 
+  matrix_of_biperm m n f 0 0 = C1.
+Proof.
+  unfold matrix_of_biperm.
+  do 2 simplify_bools_moddy_lia_one_kernel.
+  now rewrite number_preserved_0.
+Qed.
+
+Lemma matrix_of_biperm_mat_equiv_of_prop n m f g : 
+  matrix_of_biperm m n f [∝] matrix_of_biperm m n g ->
+  matrix_of_biperm m n f ≡ matrix_of_biperm m n g.
+Proof.
+  intros (c & Heq & Hc).
+  assert (Hc' : (matrix_of_biperm m n f 0 0 = 
+    c * matrix_of_biperm m n g 0 0)%C)
+  by now rewrite Heq.
+  rewrite 2!matrix_of_biperm_entry_0_0 in Hc'.
+  Csimpl_in Hc'.
+  rewrite <- Hc' in Heq.
+  rewrite Heq.
+  now rewrite Mscale_1_l.
+Qed.
+
+
+(* Lemma matrix_of_biperm_reflect_perm_grow_0_l *)
+
+Lemma compose_NF_biperms_correct' (b c : NF_biperm) n m : 
+  WF_NF_biperm b -> WF_NF_biperm c -> 
+  NF_outsize b = NF_insize c ->
+  NF_insize b = n -> NF_outsize c = m ->
+  matrix_of_biperm n m (realize_NF_biperm (compose_NF_biperms b c)) [∝]
+  @Mmult (2^n) (2^NF_insize c) (2^m) 
+    (matrix_of_NF_biperm c) (matrix_of_NF_biperm b).
+Proof.
+  intros.
+  subst n m.
+  rewrite <- (compose_NF_biperms_correct c b) by easy.
+  unfold matrix_of_NF_biperm.
+  rewrite NF_insize_compose_NF_biperms, 
+    NF_outsize_compose_NF_biperms by easy.
+  easy.
+Qed.
+
+Lemma fn_cast_eq {A} {n m n' m'} (f : forall {n m}, ZX n m -> A) (zx : ZX n m) 
+  prfn prfm : 
+  f (cast n' m' prfn prfm zx) = f zx.
+Proof.
+  now subst.
+Qed.
+
+(* FIXME: Move *)
+Create HintDb WF_NF_biperm_db discriminated.
+#[export] Hint Resolve 
+  empty_NF_biperm_WF wire_NF_biperm_WF cup_NF_biperm_WF cap_NF_biperm_WF
+  swap_NF_biperm_WF 
+  NF_of_zx_WF
+  stack_NF_biperms_WF compose_NF_biperms_WF
+  : WF_NF_biperm_db.
+
+Create HintDb zxbiperm_cleanup_db.
+#[export] Hint Rewrite @NF_insize_NF_of_zx 
+  @NF_outsize_NF_of_zx using 
+  solve [auto with zxbiperm_db] : zxbiperm_cleanup_db.
+#[export] Hint Rewrite 
+  NF_insize_stack_NF_biperms 
+  NF_outsize_stack_NF_biperms : zxbiperm_cleanup_db.
+
+Fixpoint make_n_cup_zxperm n : ZX (n * 2) (n * 2) :=
+  match n return ZX (n * 2) (n * 2) with 
+  | O => Empty
+  | S n' => 
+    (fun H G => 
+    @cast ((S n') * 2) ((S n') * 2) _ _
+      H G (— ↕ (zx_comm (n' * 2) 1))) 
+      ltac:(lia) ltac:(lia) ⟷ (n_wire 2 ↕ make_n_cup_zxperm n')
+  end.
+
+Import CoreRules.
+
+Lemma stack_split_diag {n m o p} (zx0 : ZX n m) (zx1 : ZX o p) : 
+  zx0 ↕ zx1 ∝ zx0 ↕ n_wire o ⟷ (n_wire m ↕ zx1).
+Proof.
+  now cleanup_zx.
+Qed.
+
+Lemma stack_split_antidiag {n m o p} (zx0 : ZX n m) (zx1 : ZX o p) : 
+  zx0 ↕ zx1 ∝ (n_wire n ↕ zx1) ⟷ (zx0 ↕ n_wire p).
+Proof.
+  now cleanup_zx.
+Qed.
+
+
+
+Lemma make_n_cup_zxperm_correct n : 
+  ltac:(let l := constr:((fun H G => n_cup_unswapped n ∝ 
+  cast (n + n) 0 H G (make_n_cup_zxperm n ⟷ n_stack n ⊃))
+  ltac:(lia) ltac:(lia)) in 
+  let l' := eval cbn beta in l in exact l').
+Proof.
+  induction n.
+  cbn.
+  now rewrite cast_id, compose_empty_r.
+  cbn -[Nat.add Nat.mul n_stack1].
+  rewrite compose_assoc.
+  rewrite <- (stack_compose_distr (n_wire 2) ⊃ (make_n_cup_zxperm n) (n ⇑ ⊃)).
+  apply (cast_mor (n * 2) (n * 0) (n + n) 0 ltac:(lia) ltac:(lia) _ _) in IHn.
+  clean_eqns rewrite cast_contract, cast_compose_distribute, 2!cast_id in IHn.
+  rewrite <- IHn.
+  rewrite nwire_removal_l.
+  clean_eqns rewrite cast_compose_distribute.
+  cbn [Nat.mul Nat.add]. 
+  clean_eqns simpl_rewrite (@cast_stack_distribute 2 2 0 0).
+  clean_eqns rewrite cast_id, !cast_contract.
+  rewrite (stack_split_antidiag ⊃).
+  rewrite <- compose_assoc.
+  rewrite cast_compose_l, cast_id.
+  change (n_wire 2) with (— ↕ n_wire 1).
+  rewrite <- wire_to_n_wire.
+  clean_eqns rewrite (stack_assoc — —), cast_id.
+  rewrite cast_compose_l, cast_id.
+  rewrite <- (stack_wire_distribute_l (zx_comm (n * 2) 1) 
+    (— ↕ $ n * 2, 0 ::: n_cup_unswapped n $)).
+  rewrite zx_comm_commutes_l.
+  rewrite cast_compose_distribute.
+  apply compose_simplify; [|now clean_eqns rewrite stack_empty_r, 2!cast_id].
+  rewrite (ltac:(unfold zx_comm; (clean_eqns rewrite cast_id); by_perm_eq) : zx_comm 0 1 ∝ —).
+  rewrite wire_removal_r.
+  clean_eqns rewrite cast_stack_l, cast_stack_r, cast_contract.
+  clean_eqns rewrite stack_assoc_back, cast_contract.
+  now apply cast_simplify.
+Qed.
+
+
+
+Lemma biperm_of_n_cup_unswapped n : 
+  perm_eq (n + n)
+    (biperm_of_zx (n_cup_unswapped n))
+    (reflect_perm (n + n)).
+Proof.
+  rewrite reflect_perm_defn.
+  induction n; [easy|].
+  rewrite <- Nat.add_0_r at 1.
+  apply matrix_of_biperm_inj.
+  - rewrite <- (NF_insize_NF_of_zx (n_cup_unswapped (S n))) at 1
+      by auto with zxbiperm_db.
+    pose proof (NF_outsize_NF_of_zx (n_cup_unswapped (S n)) 
+      ltac:(auto with zxbiperm_db)) as Heq.
+    rewrite <- Heq at 4.
+    apply realize_NF_biperm_bipermutation_alt.
+    apply NF_of_zx_WF; auto with zxbiperm_db.
+  - intros k Hk; lia.
+  - apply matrix_of_biperm_mat_equiv_of_prop.
+    cbn -[Nat.add].
+    rewrite compose_NF_biperms_correct' by 
+      (autorewrite with zxbiperm_cleanup_db; 
+      auto with WF_NF_biperm_db zxbiperm_db;
+      cbn; lia).
+    rewrite fn_cast_eq.
+    cbn [NF_of_zx].
+    rewrite 2!stack_NF_biperms_correct 
+      by auto with WF_NF_biperm_db zxbiperm_db.
+    rewrite matrix_of_cap_NF_biperm, matrix_of_wire_NF_biperm.
+    prop_exists_nonzero 1%R.
+    restore_dims.
+    rewrite Mscale_1_l.
+    autorewrite with zxbiperm_cleanup_db.
+    cbn -[Nat.add ZX_semantics].
+    apply mat_equiv_eq; 
+    [auto using WF_Matrix_dim_change with wf_db zarith..|].
+    apply WF_Matrix_dim_change; [lia..|].
+    apply WF_mult; [auto_wf|..].
+    repeat apply WF_kron; unify_pows_two; try lia; 
+    auto_wf.
+    autorewrite with zxbiperm_cleanup_db.
+    eapply WF_Matrix_dim_change; 
+    [..|apply matrix_of_NF_biperm_WF];
+    autorewrite with zxbiperm_cleanup_db; reflexivity.
+    unify_pows_two.
+    eapply WF_Matrix_dim_change; 
+    [..|apply matrix_of_biperm_WF];
+    cbn [Nat.add]; unify_pows_two; reflexivity.
+    apply mat_equiv_of_all_basis_conj.
+    intros i j Hi Hj.
+    cbn [Nat.add] in *.
+    unify_pows_two.
+    rewrite basis_f_to_vec_alt by (revert Hj; now unify_pows_two).
+    apply matrix_of_NF_biperm_WF.
+Abort.
+
+
+(* Lemma yank_r: forall n, n_cup n ∝ n_wire n ↕ n_swap n ⟷ n_cup_unswapped n.
+Proof.
+  intros n.
+  bdestruct (n =? 1).
+  subst.
+  unfold n_cup.
+  cbn.
+  rewrite cast_id.
+  apply ZXbiperm_prop_by_biperm_eq; [admit..|].
+  Time ZXpermAutomation.by_perm_cell; reflexivity.
+  prop_exists_nonzero 1.
+  rewrite Mscale_1_l.
+  lma'.
+Qed. *)
 
 
 
